fixing up ex3

Assignment2/Ex3.dfy
@@ -1,82 +1,86 @@
-/////////////////////////////////////////////////////////////
-//          ALL CODE IN HEADTAIL IS WRITTEN BY             //
-//                 ABANOB TAWFIK                           //
-//                    Z5075490                             //
-//                 November 2019                           //
-/////////////////////////////////////////////////////////////
-
-// Ex3.dfy 10 marks
-// In lectures, the verification of a Quack data type was shown (Week 6 lecture, slide 30). You will observe
-// that the test method for the quack calls a method called HeadTail() that is missing from the lecture
-// notes. This method swaps the data items at the two ends of the queue (so the item at the head goes
-// to the tail, and the tail goes to the head). No arguments are returned.
-// Implement this method, verifying its correctness using the ghost sequence shadow. The verified code
-// for the Quack class and its test method Main() can be found on the website.
-
-class {:autocontracts} Quack<Data>
+class Quack<Data>
 {
     var buf: array<Data>;
     var m: int, n: int;
 
     ghost var shadow: seq<Data>;
 
-    predicate Valid()
+    predicate Valid() reads this, this.buf
     { buf!=null && buf.Length!=0 && 0<=m<=n<=buf.Length && shadow==buf[m..n] }
 
-    constructor(size: int)
+    constructor(size: int) modifies this
     requires size>0;
-    ensures shadow == [];
-    ensures fresh(buf);
+    ensures shadow == []
+    ensures fresh(buf)
+    ensures Valid()
     {   buf := new Data[size];
         m, n:= 0, 0;
         shadow:= [];
     }
-
     method Empty() returns (x: bool)
     ensures x <==> shadow==[]
+    requires Valid(); ensures Valid()
     { x := m==n; }
 
-    method Pop() returns(x: Data) // + Push() works as a stack
-    requires buf != null  // version 1.9.7
+    method Pop() returns(x: Data) modifies this, this`n
+    requires buf!=null && Valid()
     requires shadow != [] 
-    ensures       x == old(shadow)[|old(shadow)|-1] // get tail
-    ensures  shadow == old(shadow)[..|old(shadow)|-1]
+    ensures Valid();
+    ensures       x  == old(shadow[|old(shadow)|-1])  // get tail
+    ensures   shadow == old(shadow[..|old(shadow)|-1])// chop off tail
+    ensures |shadow| == |old(shadow)|-1
+    ensures buf == old(buf)  // no change to buf here
     {   x, n:= buf[n-1], n-1;
         shadow:= shadow[..|shadow|-1];
     }
 
-    method Qop() returns(x: Data) // + Push() works as a queue
-    requires buf != null  // version 1.9.7
+    method Qop() returns(x: Data) modifies this, this`m
+    requires buf!=null && Valid()
     requires shadow != [];
-    ensures       x == old(shadow)[0] // get head
-    ensures  shadow == old(shadow)[1..]
+    ensures Valid();
+    ensures        x == old(shadow[0])   // get head
+    ensures   shadow == old(shadow[1..]) // chop off head
+    ensures |shadow| == |old(shadow)|-1
+    ensures buf == old(buf)  // no change to buf here
     {   x, m:= buf[m], m+1;
         shadow:= shadow[1..];
     }
 
-    method Push(x: Data)  // + Pop():a stack,  + Qop():a queue
-    requires buf != null  // version 1.9.7
-    ensures shadow == old(shadow) + [x]; // new tail
+    method Push(x: Data) modifies this, this.buf, this`m, this`n
+    requires buf!=null && Valid();
+    ensures   shadow == old(shadow) + [x]; // new tail
+    ensures |shadow| == |old(shadow)|+1
+    ensures if old(n)==old(buf.Length) then fresh(buf) else buf==old(buf)
+    ensures Valid();
     {   if n==buf.Length
-        {   var b:= new Data[buf.Length];
-            if m==0 { b:= new Data[2*buf.Length]; }
-            forall (i | 0<=i<n-m) { b[i]:= buf[m+i]; }
-            buf, m, n:= b, 0, n-m;
+        {   var b:= new Data[buf.Length];             // temporary
+            if m==0 { b:= new Data[2*buf.Length]; }   // double size
+            forall (i | 0<=i<n-m) { b[i]:= buf[m+i]; }// copy m..n to 0..n-m
+            buf, m, n:= b, 0, n-m;                    // copy b to buf, reset m,n
         }
-        buf[n], n:= x, n+1;
-        shadow:= shadow + [x];
+        buf[n], n:= x, n+1;         // now we definitely have room
+        shadow:= shadow + [x];      // same as previous slide: concat 'x'
     }   
 
-    method HeadTail()
+    method HeadTail()  modifies this.buf,  this`shadow
     requires buf != null  // version 1.9.7
+    requires Valid() 
     // no change in size
+    ensures n == old(n)
+    ensures m == old(m)
     ensures |shadow| == |old(shadow)|
+    ensures buf.Length == old(buf).Length
     // if the size of our quack is between 0 and 2, then we just leave it alone
     // headtail for 0 or 1 element should do nothing
-    ensures !(n - m >= 2) ==> shadow == old(shadow)
     // we take the tail and make it the head, append everything else to the array, then we take the head and make it the tail
-    // this also ensures nothing else changes but head/tail
-    ensures (n - m >= 2) ==> shadow == old(shadow[|old(shadow)| - 1..]) + old(shadow[1..|old(shadow)| - 1]) + old(shadow[0..1])
+    ensures (|shadow| >= 2) ==> shadow == old(shadow[|old(shadow)| - 1..]) + old(shadow[1..|old(shadow)| - 1]) + old(shadow[0..1])
+    // everything between head and tails stay same, hence the < instead of <= 
+    ensures (|shadow| >= 2) ==> (forall i :: m < i < n - 1 ==> (buf[i] == old(buf[i]))) && (buf[m] == old(buf[n - 1]) && buf[n - 1] == old(buf[m]))
+    ensures (|shadow| < 2) ==> buf == old(buf)
+    ensures (|shadow| < 2) ==> shadow == old(shadow)
+    // ensures multiset(shadow) == multiset(old(shadow)) && multiset(buf[..]) == multiset(old(buf[..]))
+    ensures Valid()
+    // ensures (n - m >= 2) ==> shadow == old(shadow[|old(shadow)| - 1..]) + old(shadow[1..|old(shadow)| - 1]) + old(shadow[0..1])
     {
         // only do anything if our quack is of size bigger than 2, (n - m) is size of the array
         if n - m >= 2 
@@ -91,17 +95,18 @@ class {:autocontracts} Quack<Data>
     }
 } // end of Quack class
 
-method Main()
+method Main() // Dafny 1.9.7
 {   var q:= new Quack<char>(10);
     var l: char;
     q.Push('r'); q.Push('s'); q.Push('k'); q.Push('o'); q.Push('w');
-    l:= q.Pop(); print l;  
+    l:= q.Pop(); assert l=='w'; print l;  
     q.HeadTail();
-    l:= q.Qop(); print l;
-    l:= q.Pop(); print l;
+    l:= q.Qop(); assert l=='o'; print l;
+    l:= q.Pop(); assert l=='r'; print l;
     q.HeadTail();
-    l:= q.Qop(); print l;    
-    l:= q.Qop(); print l;        
+    l:= q.Qop(); assert l=='k'; print l;    
+    q.HeadTail();
+    l:= q.Qop(); assert l=='s'; print l;        
     var e: bool:= q.Empty();
     if e {print "\nqueue empty\n";} else {print "\nqueue not empty\n";}
 }
